Split Uniform into UniformPowerOfTwo and Uniform (#43)
* Split Uniform into UniformPowerOfTwo and Uniform

* Rename Unif -> UniformPowerOfTwo in public names

* fix

* fix

src/Distributions/Uniform/Model.dfy
@@ -8,6 +8,7 @@ include "../../ProbabilisticProgramming/Monad.dfy"
 include "../../ProbabilisticProgramming/Independence.dfy"
 include "../../ProbabilisticProgramming/Quantifier.dfy"
 include "../../ProbabilisticProgramming/WhileAndUntil.dfy"
+include "../UniformPowerOfTwo/Model.dfy"
 
 module UniformModel {
   import opened RandomNumberGenerator
@@ -15,18 +16,7 @@ module UniformModel {
   import opened Monad
   import opened Independence
   import opened WhileAndUntil
-
-  // Definition 48
-  function ProbUnif(n: nat): (h: Hurd<nat>) {
-    if n == 0 then
-      Return(0)
-    else
-      var f := (m: nat) =>
-                  var g := (b: bool) =>
-                            Return(if b then 2*m + 1 else 2*m);
-                  Bind(Deconstruct, g);
-      Bind(ProbUnif(n/2), f)
-  }
+  import opened UniformPowerOfTwoModel
 
   // Definition 49
   function ProbUniform(n: nat): Hurd<nat>
@@ -44,74 +34,10 @@ module UniformModel {
       (a + x, s')
   }
 
-  lemma {:axiom} ProbUnifTerminates(n: nat)
-    requires n > 0
-    ensures
-      var b := ProbUnif(n - 1);
-      var c := (x: nat) => x < n;
-      && IsIndepFn(b)
-      && ExistsStar(Helper2(b, c))
-      && ProbUntilTerminates(b, c)
-
-  function ProbUnifAlternative(n: nat, s: RNG, k: nat := 1, u: nat := 0): (t: (nat, RNG))
-    requires k >= 1
-    decreases 2*n - k
-  {
-    if k > n then
-      (u, s)
-    else
-      ProbUnifAlternative(n, Tail(s), 2*k, if Head(s) then 2*u + 1 else 2*u)
-  }
-
-  function UnifAlternativeModel(n: nat, k: nat := 1, u: nat := 0): Hurd<nat>
-    requires k >= 1
-  {
-    (s: RNG) => ProbUnifAlternative(n, s, k, u)
-  }
-
-  function UnifModel(n: nat): (f: Hurd<nat>)
-    ensures forall s :: f(s) == UnifAlternativeModel(n)(s)
-  {
-    var f := ProbUnif(n);
-    assert forall s :: f(s) == UnifAlternativeModel(n)(s) by {
-      forall s ensures f(s) == UnifAlternativeModel(n)(s) {
-        ProbUnifCorrespondence(n, s);
-      }
-    }
-    f
-  }
-
   function UniformIntervalModel(a: int, b: int): (f: Hurd<int>)
     requires a < b
     ensures forall s :: f(s).0 == a + ProbUniform(b - a)(s).0
   {
     ProbUniformInterval(a, b)
-  }
-
-  lemma ProbUnifCorrespondence(n: nat, s: RNG)
-    ensures ProbUnifAlternative(n, s) == ProbUnif(n)(s)
-  {
-    var f := (m: nat) =>
-        var g := (b: bool) =>
-                   Return(if b then 2*m + 1 else 2*m);
-        Bind(Deconstruct, g);
-    if n == 0 {
-    } else if n == 1 {
-      assert n / 2 == 0;
-      assert (0, s) == ProbUnif(n/2)(s);
-      calc {
-        ProbUnif(n)(s);
-        Bind(ProbUnif(n/2), f)(s);
-        f(0)(s);
-        Bind(Deconstruct, (b: bool) => Return(if b then 1 else 0))(s);
-        Return(if Head(s) then 1 else 0)(Tail(s));
-        (if Head(s) then 1 else 0, Tail(s));
-        ProbUnifAlternative(1, Tail(s), 2, if Head(s) then 1 else 0);
-        ProbUnifAlternative(1, s, 1, 0);
-        ProbUnifAlternative(n, s);
-      }
-    } else {
-      assume {:axiom} false;
-    }
   }
 }
