src/Distributions/UniformPowerOfTwo/Implementation.dfy
@@ -1,0 +1,36 @@
+/*******************************************************************************
+*  Copyright by the contributors to the Dafny Project
+*  SPDX-License-Identifier: MIT
+*******************************************************************************/
+
+include "../../Math/MeasureTheory.dfy"
+include "../../ProbabilisticProgramming/Monad.dfy"
+include "Interface.dfy"
+include "Model.dfy"
+
+module UniformPowerOfTwoImplementation {
+  import opened MeasureTheory
+  import opened Monad
+  import opened UniformPowerOfTwoModel
+  import opened UniformPowerOfTwoInterface
+
+  trait {:termination false} TUniformPowerOfTwo extends IUniformPowerOfTwo {
+    method UniformPowerOfTwo(n: nat) returns (u: nat)
+      modifies this
+      ensures UniformPowerOfTwoModel.UnifModel(n)(old(s)) == (u, s)
+    {
+      var k := 1;
+      u := 0;
+
+      while k <= n
+        decreases 2*n - k
+        invariant k >= 1
+        invariant UnifAlternativeModel(n)(old(s)) == UnifAlternativeModel(n, k, u)(s)
+      {
+        var b := Coin();
+        k := 2*k;
+        u := if b then 2*u + 1 else 2*u;
+      }
+    }
+  }
+}
