src/Distributions/UniformPowerOfTwo/Interface.dfy
@@ -1,0 +1,20 @@
+/*******************************************************************************
+*  Copyright by the contributors to the Dafny Project
+*  SPDX-License-Identifier: MIT
+*******************************************************************************/
+
+include "../Base/Interface.dfy"
+include "Model.dfy"
+
+module UniformPowerOfTwoInterface {
+  import opened BaseInterface
+  import opened UniformPowerOfTwoModel
+
+  trait {:termination false} IUniformPowerOfTwo extends TBase {
+
+    method UniformPowerOfTwo(n: nat) returns (u: nat)
+      modifies this
+      ensures UniformPowerOfTwoModel.ProbUnif(n)(old(s)) == (u, s)
+
+  }
+}
