src/Distributions/UniformPowerOfTwo/Model.dfy
@@ -1,0 +1,94 @@
+/*******************************************************************************
+*  Copyright by the contributors to the Dafny Project
+*  SPDX-License-Identifier: MIT
+*******************************************************************************/
+
+include "../../ProbabilisticProgramming/RandomNumberGenerator.dfy"
+include "../../ProbabilisticProgramming/Monad.dfy"
+include "../../ProbabilisticProgramming/Independence.dfy"
+include "../../ProbabilisticProgramming/Quantifier.dfy"
+include "../../ProbabilisticProgramming/WhileAndUntil.dfy"
+
+module UniformPowerOfTwoModel {
+  import opened RandomNumberGenerator
+  import opened Quantifier
+  import opened Monad
+  import opened Independence
+  import opened WhileAndUntil
+
+  // Definition 48
+  function ProbUnif(n: nat): (h: Hurd<nat>) {
+    if n == 0 then
+      Return(0)
+    else
+      var f := (m: nat) =>
+                  var g := (b: bool) =>
+                            Return(if b then 2*m + 1 else 2*m);
+                  Bind(Deconstruct, g);
+      Bind(ProbUnif(n/2), f)
+  }
+
+  lemma {:axiom} ProbUnifTerminates(n: nat)
+    requires n > 0
+    ensures
+      var b := ProbUnif(n - 1);
+      var c := (x: nat) => x < n;
+      && IsIndepFn(b)
+      && ExistsStar(Helper2(b, c))
+      && ProbUntilTerminates(b, c)
+
+  function ProbUnifAlternative(n: nat, s: RNG, k: nat := 1, u: nat := 0): (t: (nat, RNG))
+    requires k >= 1
+    decreases 2*n - k
+  {
+    if k > n then
+      (u, s)
+    else
+      ProbUnifAlternative(n, Tail(s), 2*k, if Head(s) then 2*u + 1 else 2*u)
+  }
+
+  function UnifAlternativeModel(n: nat, k: nat := 1, u: nat := 0): Hurd<nat>
+    requires k >= 1
+  {
+    (s: RNG) => ProbUnifAlternative(n, s, k, u)
+  }
+
+  function UnifModel(n: nat): (f: Hurd<nat>)
+    ensures forall s :: f(s) == UnifAlternativeModel(n)(s)
+  {
+    var f := ProbUnif(n);
+    assert forall s :: f(s) == UnifAlternativeModel(n)(s) by {
+      forall s ensures f(s) == UnifAlternativeModel(n)(s) {
+        ProbUnifCorrespondence(n, s);
+      }
+    }
+    f
+  }
+
+  lemma ProbUnifCorrespondence(n: nat, s: RNG)
+    ensures ProbUnifAlternative(n, s) == ProbUnif(n)(s)
+  {
+    var f := (m: nat) =>
+        var g := (b: bool) =>
+                   Return(if b then 2*m + 1 else 2*m);
+        Bind(Deconstruct, g);
+    if n == 0 {
+    } else if n == 1 {
+      assert n / 2 == 0;
+      assert (0, s) == ProbUnif(n/2)(s);
+      calc {
+        ProbUnif(n)(s);
+        Bind(ProbUnif(n/2), f)(s);
+        f(0)(s);
+        Bind(Deconstruct, (b: bool) => Return(if b then 1 else 0))(s);
+        Return(if Head(s) then 1 else 0)(Tail(s));
+        (if Head(s) then 1 else 0, Tail(s));
+        ProbUnifAlternative(1, Tail(s), 2, if Head(s) then 1 else 0);
+        ProbUnifAlternative(1, s, 1, 0);
+        ProbUnifAlternative(n, s);
+      }
+    } else {
+      assume {:axiom} false;
+    }
+  }
+}
